NuSys.thy
@@ -141,10 +141,10 @@ lemma \<phi>reassemble_proc_final:
   by (metis StrictStateTy_intro(1) state.simps(15))
 
 
-lemma \<phi>rename_proc: "f \<equiv> f' \<Longrightarrow> \<^bold>p\<^bold>r\<^bold>o\<^bold>c f' \<lbrace> U \<longmapsto> \<R> \<rbrace> \<Longrightarrow> \<^bold>p\<^bold>r\<^bold>o\<^bold>c f \<lbrace> U \<longmapsto> \<R> \<rbrace>" by fast
+lemma \<phi>rename_proc: "f \<equiv> f' \<Longrightarrow> \<^bold>p\<^bold>r\<^bold>o\<^bold>c f' \<lbrace> U \<longmapsto> \<R> \<^bold>t\<^bold>h\<^bold>r\<^bold>o\<^bold>w\<^bold>s E \<rbrace> \<Longrightarrow> \<^bold>p\<^bold>r\<^bold>o\<^bold>c f \<lbrace> U \<longmapsto> \<R> \<^bold>t\<^bold>h\<^bold>r\<^bold>o\<^bold>w\<^bold>s E \<rbrace>" by fast
 
 lemma \<phi>rename_proc_with_goal:
-  \<open>f \<equiv> f' \<Longrightarrow> \<^bold>p\<^bold>r\<^bold>o\<^bold>c f' \<lbrace> U \<longmapsto> \<R> \<rbrace> \<^bold>@\<^bold>G\<^bold>O\<^bold>A\<^bold>L G \<Longrightarrow> \<^bold>p\<^bold>r\<^bold>o\<^bold>c f \<lbrace> U \<longmapsto> \<R> \<rbrace> \<^bold>@\<^bold>G\<^bold>O\<^bold>A\<^bold>L G\<close>
+  \<open>f \<equiv> f' \<Longrightarrow> \<^bold>p\<^bold>r\<^bold>o\<^bold>c f' \<lbrace> U \<longmapsto> \<R> \<^bold>t\<^bold>h\<^bold>r\<^bold>o\<^bold>w\<^bold>s E \<rbrace> \<^bold>@\<^bold>G\<^bold>O\<^bold>A\<^bold>L G \<Longrightarrow> \<^bold>p\<^bold>r\<^bold>o\<^bold>c f \<lbrace> U \<longmapsto> \<R> \<^bold>t\<^bold>h\<^bold>r\<^bold>o\<^bold>w\<^bold>s E \<rbrace> \<^bold>@\<^bold>G\<^bold>O\<^bold>A\<^bold>L G\<close>
   unfolding GOAL_CTXT_def using \<phi>rename_proc .
 
 
@@ -341,6 +341,22 @@ lemma [\<phi>reason 1200 on \<open>lambda_abstraction (tag ?x) ?fx ?f\<close>]:
 \<Longrightarrow> rename_abstraction TYPE('name) f f'
 \<Longrightarrow> lambda_abstraction (tag x :: 'any <named> 'name) fx (case_named f')\<close>
   unfolding lambda_abstraction_def rename_abstraction_def by simp
+
+
+subsubsection \<open>Extract Proof Obligation\<close>
+
+lemma contract_obligations:
+  "(Premise mode P \<Longrightarrow> \<^bold>o\<^bold>b\<^bold>l\<^bold>i\<^bold>g\<^bold>a\<^bold>t\<^bold>i\<^bold>o\<^bold>n Q \<Longrightarrow> PROP C) \<equiv> (\<^bold>o\<^bold>b\<^bold>l\<^bold>i\<^bold>g\<^bold>a\<^bold>t\<^bold>i\<^bold>o\<^bold>n P \<and> Q \<Longrightarrow> PROP C)"
+  unfolding Premise_def atomize_imp conj_imp .
+
+ML_file "library/reasoners.ML"
+
+\<phi>reasoner_ML Normal_Premise 10 (conclusion \<open>\<^bold>p\<^bold>r\<^bold>e\<^bold>m\<^bold>i\<^bold>s\<^bold>e ?P\<close> | conclusion \<open>\<^bold>o\<^bold>b\<^bold>l\<^bold>i\<^bold>g\<^bold>a\<^bold>t\<^bold>i\<^bold>o\<^bold>n ?P\<close>)
+  = \<open>Nu_Reasoners.wrap Nu_Reasoners.premise_tac\<close>
+\<phi>reasoner  Simp_Premise 10 (conclusion \<open>\<^bold>s\<^bold>i\<^bold>m\<^bold>p\<^bold>r\<^bold>e\<^bold>m ?P\<close>)
+  = (rule Premise_I; simp; fail)
+\<phi>reasoner \<phi>expn_Premise 10 (conclusion \<open><\<phi>expn> ?P\<close>)
+  = (rule Premise_I; simp add: \<phi>expns)
 
 
 
@@ -1013,6 +1029,19 @@ lemma \<phi>application_success:
   \<open>PROP \<phi>Application_Success\<close>
   unfolding \<phi>Application_Success_def ..
 
+
+definition \<phi>Application_Conv :: \<open>prop \<Rightarrow> prop \<Rightarrow> prop\<close>
+  where \<open>\<phi>Application_Conv P Q \<equiv> (PROP P \<Longrightarrow> PROP Q)\<close>
+
+lemma \<phi>Application_Conv:
+  \<open> PROP P
+\<Longrightarrow> PROP \<phi>Application_Conv P Q
+\<Longrightarrow> \<r>Success
+\<Longrightarrow> \<^bold>o\<^bold>b\<^bold>l\<^bold>i\<^bold>g\<^bold>a\<^bold>t\<^bold>i\<^bold>o\<^bold>n True
+\<Longrightarrow> PROP Q\<close>
+  unfolding \<phi>Application_Conv_def .
+
+
 ML_file \<open>library/application.ML\<close>
 
 \<phi>reasoner_ML \<phi>Application 2000 (conclusion \<open>(PROP ?App) \<^bold>a\<^bold>p\<^bold>p\<^bold>l\<^bold>i\<^bold>e\<^bold>s ?State \<^bold>\<Rightarrow> (PROP ?Result)\<close>) =
@@ -1084,21 +1113,12 @@ lemma [\<phi>reason 1200]:
   subgoal premises prems using prems(1)[OF prems(2) prems(3)] . .
 
 
-definition \<phi>Application_Conv :: \<open>prop \<Rightarrow> prop \<Rightarrow> prop\<close>
-  where \<open>\<phi>Application_Conv P Q \<equiv> (PROP P \<Longrightarrow> PROP Q)\<close>
-
 lemma [\<phi>reason 1200]:
   \<open> PROP \<phi>Application_Conv X' X
 \<Longrightarrow> PROP \<phi>Application_Success
 \<Longrightarrow> PROP \<phi>Application_Method X' (PROP X \<Longrightarrow> PROP Y) Y\<close>
   unfolding \<phi>Application_Method_def \<phi>Application_def \<phi>Application_Conv_def
   subgoal premises prems using prems(3)[OF prems(1)[OF prems(4)]] . .
-
-lemma \<phi>Application_Conv:
-  \<open> PROP P
-\<Longrightarrow> PROP \<phi>Application_Conv P Q
-\<Longrightarrow> PROP Q\<close>
-  unfolding \<phi>Application_Conv_def .
 
 lemma [\<phi>reason 1200]:
   \<open> PROP \<phi>Application_Conv (Trueprop X') (Trueprop X)
@@ -1307,7 +1327,7 @@ in
         = strip [] (hd (Thm.prems_of sequent))
     in (case Term.strip_comb (Envir.beta_eta_contract f') of (Var v, args) =>
          Thm.instantiate (TVars.empty, Vars.make [
-              (v, Thm.cterm_of ctxt (fold (my_abstract_over btys) args f))]) sequent
+              (v, Thm.cterm_of ctxt (fold_rev (my_abstract_over btys) args f))]) sequent
         | _ => sequent)
        |> (fn seq => Seq.single (ctxt, @{thm Exhaustive_Abstract_I} RS seq))
     end
@@ -1805,23 +1825,6 @@ lemma [\<phi>reason 1000]: "SameNuTy A A" \<comment> \<open>The fallback\<close>
   unfolding SameNuTy_def ..
 
 
-subsubsection \<open>Extract Proof Obligation\<close>
-
-lemma contract_obligations:
-  "(Premise mode P \<Longrightarrow> \<^bold>o\<^bold>b\<^bold>l\<^bold>i\<^bold>g\<^bold>a\<^bold>t\<^bold>i\<^bold>o\<^bold>n Q \<Longrightarrow> PROP C) \<equiv> (\<^bold>o\<^bold>b\<^bold>l\<^bold>i\<^bold>g\<^bold>a\<^bold>t\<^bold>i\<^bold>o\<^bold>n P \<and> Q \<Longrightarrow> PROP C)"
-  unfolding Premise_def atomize_imp conj_imp .
-
-ML_file "library/reasoners.ML"
-
-\<phi>reasoner_ML Normal_Premise 10 (conclusion \<open>\<^bold>p\<^bold>r\<^bold>e\<^bold>m\<^bold>i\<^bold>s\<^bold>e ?P\<close> | conclusion \<open>\<^bold>o\<^bold>b\<^bold>l\<^bold>i\<^bold>g\<^bold>a\<^bold>t\<^bold>i\<^bold>o\<^bold>n ?P\<close>)
-  = \<open>Nu_Reasoners.wrap Nu_Reasoners.premise_tac\<close>
-\<phi>reasoner  Simp_Premise 10 (conclusion \<open>\<^bold>s\<^bold>i\<^bold>m\<^bold>p\<^bold>r\<^bold>e\<^bold>m ?P\<close>)
-  = (rule Premise_I; simp; fail)
-\<phi>reasoner \<phi>expn_Premise 10 (conclusion \<open><\<phi>expn> ?P\<close>)
-  = (rule Premise_I; simp add: \<phi>expns)
-
-
-
 subsection \<open>Subty Reasoning\<close>
 
 lemmas cast_def = GOAL_CTXT_def FOCUS_TAG_def Subty_def
@@ -1837,9 +1840,9 @@ lemmas cast_def = GOAL_CTXT_def FOCUS_TAG_def Subty_def
 
 subsubsection \<open>Identity Subty\<close>
 
-lemma [\<phi>reason 3000 on \<open>\<^bold>s\<^bold>u\<^bold>b\<^bold>t\<^bold>y\<^bold>p\<^bold>e ?H \<longmapsto> \<blangle> ?H2 \<brangle> \<^bold>w\<^bold>i\<^bold>t\<^bold>h ?P \<^bold>@\<^bold>G\<^bold>O\<^bold>A\<^bold>L ?G\<close>]:
+lemma [\<phi>reason 4000 on \<open>\<^bold>s\<^bold>u\<^bold>b\<^bold>t\<^bold>y\<^bold>p\<^bold>e ?H \<longmapsto> \<blangle> ?H2 \<brangle> \<^bold>w\<^bold>i\<^bold>t\<^bold>h ?P \<^bold>@\<^bold>G\<^bold>O\<^bold>A\<^bold>L ?G\<close>]:
       "\<^bold>s\<^bold>u\<^bold>b\<^bold>t\<^bold>y\<^bold>p\<^bold>e H \<longmapsto> \<blangle> H \<brangle>  \<^bold>@\<^bold>G\<^bold>O\<^bold>A\<^bold>L G"
-  and [\<phi>reason 3000 on \<open>\<^bold>s\<^bold>u\<^bold>b\<^bold>t\<^bold>y\<^bold>p\<^bold>e ?H \<longmapsto> ?R * \<blangle> ?H2 \<brangle> \<^bold>w\<^bold>i\<^bold>t\<^bold>h ?P \<^bold>@\<^bold>G\<^bold>O\<^bold>A\<^bold>L ?G\<close>]:
+  and [\<phi>reason 4000 on \<open>\<^bold>s\<^bold>u\<^bold>b\<^bold>t\<^bold>y\<^bold>p\<^bold>e ?H \<longmapsto> ?R * \<blangle> ?H2 \<brangle> \<^bold>w\<^bold>i\<^bold>t\<^bold>h ?P \<^bold>@\<^bold>G\<^bold>O\<^bold>A\<^bold>L ?G\<close>]:
       "\<^bold>s\<^bold>u\<^bold>b\<^bold>t\<^bold>y\<^bold>p\<^bold>e H \<longmapsto> 1 * \<blangle> H \<brangle>  \<^bold>@\<^bold>G\<^bold>O\<^bold>A\<^bold>L G"
   for H :: \<open>'a::monoid_mult set\<close>
   unfolding cast_def mult_1_left by blast+
@@ -1877,13 +1880,19 @@ subsubsection \<open>Pad 1 Holes at left\<close> \<comment> \<open>to standardiz
 
 lemma [\<phi>reason 2000
   if no \<open>\<^bold>s\<^bold>u\<^bold>b\<^bold>t\<^bold>y\<^bold>p\<^bold>e ?H \<longmapsto> \<blangle> (?X1 \<heavy_comma> ?X2) \<brangle> \<^bold>w\<^bold>i\<^bold>t\<^bold>h ?P \<^bold>@\<^bold>G\<^bold>O\<^bold>A\<^bold>L ?G\<close>
-        \<open>\<^bold>s\<^bold>u\<^bold>b\<^bold>t\<^bold>y\<^bold>p\<^bold>e ?H \<longmapsto> \<blangle> Void \<brangle> \<^bold>w\<^bold>i\<^bold>t\<^bold>h ?P \<^bold>@\<^bold>G\<^bold>O\<^bold>A\<^bold>L ?G\<close>]:
+        \<open>\<^bold>s\<^bold>u\<^bold>b\<^bold>t\<^bold>y\<^bold>p\<^bold>e ?H \<longmapsto> \<blangle> ?X1 + ?X2 \<brangle> \<^bold>w\<^bold>i\<^bold>t\<^bold>h ?P \<^bold>@\<^bold>G\<^bold>O\<^bold>A\<^bold>L ?G\<close>
+        \<open>\<^bold>s\<^bold>u\<^bold>b\<^bold>t\<^bold>y\<^bold>p\<^bold>e ?H \<longmapsto> \<blangle> 1 \<brangle> \<^bold>w\<^bold>i\<^bold>t\<^bold>h ?P \<^bold>@\<^bold>G\<^bold>O\<^bold>A\<^bold>L ?G\<close>]:
   "\<^bold>s\<^bold>u\<^bold>b\<^bold>t\<^bold>y\<^bold>p\<^bold>e H \<longmapsto> \<blangle> 1 \<heavy_comma> X \<brangle> \<^bold>w\<^bold>i\<^bold>t\<^bold>h P \<^bold>@\<^bold>G\<^bold>O\<^bold>A\<^bold>L G \<Longrightarrow>
    \<^bold>s\<^bold>u\<^bold>b\<^bold>t\<^bold>y\<^bold>p\<^bold>e H \<longmapsto> \<blangle> X \<brangle> \<^bold>w\<^bold>i\<^bold>t\<^bold>h P \<^bold>@\<^bold>G\<^bold>O\<^bold>A\<^bold>L G"
   unfolding cast_def mult_1_left .
 
 lemma [\<phi>reason 2000
     if no \<open>\<^bold>s\<^bold>u\<^bold>b\<^bold>t\<^bold>y\<^bold>p\<^bold>e ?Y1 \<heavy_comma> ?Y2 \<longmapsto> ?X \<^bold>w\<^bold>i\<^bold>t\<^bold>h ?P \<^bold>@\<^bold>G\<^bold>O\<^bold>A\<^bold>L ?G\<close>
+          \<open>\<^bold>s\<^bold>u\<^bold>b\<^bold>t\<^bold>y\<^bold>p\<^bold>e ?Y1 + ?Y2 \<longmapsto> ?X \<^bold>w\<^bold>i\<^bold>t\<^bold>h ?P \<^bold>@\<^bold>G\<^bold>O\<^bold>A\<^bold>L ?G\<close>
+          \<open>\<^bold>s\<^bold>u\<^bold>b\<^bold>t\<^bold>y\<^bold>p\<^bold>e 1 \<longmapsto> ?X \<^bold>w\<^bold>i\<^bold>t\<^bold>h ?P \<^bold>@\<^bold>G\<^bold>O\<^bold>A\<^bold>L ?G\<close>
+          \<open>\<^bold>s\<^bold>u\<^bold>b\<^bold>t\<^bold>y\<^bold>p\<^bold>e ?H \<longmapsto> \<blangle> ?X1 + ?X2 \<brangle> \<^bold>w\<^bold>i\<^bold>t\<^bold>h ?P \<^bold>@\<^bold>G\<^bold>O\<^bold>A\<^bold>L ?G\<close>
+          \<open>\<^bold>s\<^bold>u\<^bold>b\<^bold>t\<^bold>y\<^bold>p\<^bold>e ?H \<longmapsto> \<blangle> 1 \<brangle> \<^bold>w\<^bold>i\<^bold>t\<^bold>h ?P \<^bold>@\<^bold>G\<^bold>O\<^bold>A\<^bold>L ?G\<close>
+          \<open>\<^bold>s\<^bold>u\<^bold>b\<^bold>t\<^bold>y\<^bold>p\<^bold>e ?H \<longmapsto> \<blangle> 0 \<brangle> \<^bold>w\<^bold>i\<^bold>t\<^bold>h ?P \<^bold>@\<^bold>G\<^bold>O\<^bold>A\<^bold>L ?G\<close>
 ]:
   "\<^bold>s\<^bold>u\<^bold>b\<^bold>t\<^bold>y\<^bold>p\<^bold>e 1 \<heavy_comma> Y \<longmapsto> X \<^bold>w\<^bold>i\<^bold>t\<^bold>h P \<^bold>@\<^bold>G\<^bold>O\<^bold>A\<^bold>L G \<Longrightarrow>
    \<^bold>s\<^bold>u\<^bold>b\<^bold>t\<^bold>y\<^bold>p\<^bold>e Y \<longmapsto> X \<^bold>w\<^bold>i\<^bold>t\<^bold>h P \<^bold>@\<^bold>G\<^bold>O\<^bold>A\<^bold>L G"
@@ -1937,7 +1946,8 @@ lemma [\<phi>intro 1100]: \<comment> \<open>tail the step\<close>
 
 subsubsection \<open>Zero\<close>
 
-lemma [\<phi>reason 3000 on \<open>\<^bold>s\<^bold>u\<^bold>b\<^bold>t\<^bold>y\<^bold>p\<^bold>e 0 \<longmapsto> ?X \<^bold>w\<^bold>i\<^bold>t\<^bold>h ?P \<^bold>@\<^bold>G\<^bold>O\<^bold>A\<^bold>L ?G\<close>]:
+lemma [\<phi>reason 3000 on \<open>\<^bold>s\<^bold>u\<^bold>b\<^bold>t\<^bold>y\<^bold>p\<^bold>e 0 \<longmapsto> ?X \<^bold>w\<^bold>i\<^bold>t\<^bold>h ?P \<^bold>@\<^bold>G\<^bold>O\<^bold>A\<^bold>L ?G\<close>
+                       \<open>\<^bold>s\<^bold>u\<^bold>b\<^bold>t\<^bold>y\<^bold>p\<^bold>e ?var_Y \<longmapsto> ?X \<^bold>w\<^bold>i\<^bold>t\<^bold>h ?P \<^bold>@\<^bold>G\<^bold>O\<^bold>A\<^bold>L ?G\<close>]:
   \<open>\<^bold>s\<^bold>u\<^bold>b\<^bold>t\<^bold>y\<^bold>p\<^bold>e 0 \<longmapsto> X \<^bold>@\<^bold>G\<^bold>O\<^bold>A\<^bold>L G\<close>
   unfolding cast_def zero_set_def by simp
 
@@ -1954,10 +1964,24 @@ subsubsection \<open>Union\<close>
 
 lemma [\<phi>reason 2500 on \<open>\<^bold>s\<^bold>u\<^bold>b\<^bold>t\<^bold>y\<^bold>p\<^bold>e ?A + ?B \<longmapsto> ?X \<^bold>w\<^bold>i\<^bold>t\<^bold>h ?P \<^bold>@\<^bold>G\<^bold>O\<^bold>A\<^bold>L ?G\<close>]:
   \<open> SUBGOAL G G1
-\<Longrightarrow> \<^bold>s\<^bold>u\<^bold>b\<^bold>t\<^bold>y\<^bold>p\<^bold>e B \<longmapsto> X \<^bold>w\<^bold>i\<^bold>t\<^bold>h P \<^bold>@\<^bold>G\<^bold>O\<^bold>A\<^bold>L G1
+\<Longrightarrow> \<^bold>s\<^bold>u\<^bold>b\<^bold>t\<^bold>y\<^bold>p\<^bold>e B \<longmapsto> X \<^bold>w\<^bold>i\<^bold>t\<^bold>h P1 \<^bold>@\<^bold>G\<^bold>O\<^bold>A\<^bold>L G1
 \<Longrightarrow> SOLVE_SUBGOAL G1
-\<Longrightarrow> \<^bold>s\<^bold>u\<^bold>b\<^bold>t\<^bold>y\<^bold>p\<^bold>e A \<longmapsto> X \<^bold>w\<^bold>i\<^bold>t\<^bold>h P \<^bold>@\<^bold>G\<^bold>O\<^bold>A\<^bold>L G
-\<Longrightarrow> \<^bold>s\<^bold>u\<^bold>b\<^bold>t\<^bold>y\<^bold>p\<^bold>e A + B \<longmapsto> X \<^bold>w\<^bold>i\<^bold>t\<^bold>h P \<^bold>@\<^bold>G\<^bold>O\<^bold>A\<^bold>L G\<close>
+\<Longrightarrow> \<^bold>s\<^bold>u\<^bold>b\<^bold>t\<^bold>y\<^bold>p\<^bold>e A \<longmapsto> X \<^bold>w\<^bold>i\<^bold>t\<^bold>h P2 \<^bold>@\<^bold>G\<^bold>O\<^bold>A\<^bold>L G
+\<Longrightarrow> \<^bold>s\<^bold>u\<^bold>b\<^bold>t\<^bold>y\<^bold>p\<^bold>e A + B \<longmapsto> X \<^bold>w\<^bold>i\<^bold>t\<^bold>h P1 \<or> P2 \<^bold>@\<^bold>G\<^bold>O\<^bold>A\<^bold>L G\<close>
+  unfolding cast_def plus_set_def by simp
+
+lemma [\<phi>reason 800]:
+  \<open> SUBGOAL G G1
+\<Longrightarrow> \<^bold>s\<^bold>u\<^bold>b\<^bold>t\<^bold>y\<^bold>p\<^bold>e X \<longmapsto> \<blangle> A \<brangle> \<^bold>w\<^bold>i\<^bold>t\<^bold>h P \<^bold>@\<^bold>G\<^bold>O\<^bold>A\<^bold>L G1
+\<Longrightarrow> SOLVE_SUBGOAL G1
+\<Longrightarrow> \<^bold>s\<^bold>u\<^bold>b\<^bold>t\<^bold>y\<^bold>p\<^bold>e X \<longmapsto> \<blangle> A + B \<brangle> \<^bold>w\<^bold>i\<^bold>t\<^bold>h P \<^bold>@\<^bold>G\<^bold>O\<^bold>A\<^bold>L G\<close>
+  unfolding cast_def plus_set_def by simp
+
+lemma [\<phi>reason 800]:
+  \<open> SUBGOAL G G1
+\<Longrightarrow> \<^bold>s\<^bold>u\<^bold>b\<^bold>t\<^bold>y\<^bold>p\<^bold>e X \<longmapsto> \<blangle> B \<brangle> \<^bold>w\<^bold>i\<^bold>t\<^bold>h P \<^bold>@\<^bold>G\<^bold>O\<^bold>A\<^bold>L G1
+\<Longrightarrow> SOLVE_SUBGOAL G1
+\<Longrightarrow> \<^bold>s\<^bold>u\<^bold>b\<^bold>t\<^bold>y\<^bold>p\<^bold>e X \<longmapsto> \<blangle> A + B \<brangle> \<^bold>w\<^bold>i\<^bold>t\<^bold>h P \<^bold>@\<^bold>G\<^bold>O\<^bold>A\<^bold>L G\<close>
   unfolding cast_def plus_set_def by simp
 
 subsubsection \<open>General\<close>
@@ -2584,7 +2608,7 @@ subsubsection \<open>Constructive\<close>
 \<phi>processor set_label 5000 (\<open>\<^bold>l\<^bold>a\<^bold>b\<^bold>e\<^bold>l ?P \<Longrightarrow> PROP ?Q\<close>) \<open>fn stat => Parse.name >> (fn name => fn _ =>
   NuSys.set_label name stat)\<close>
 
-\<phi>processor rule 9000 (\<open>?P \<Longrightarrow> PROP ?Q\<close>)
+\<phi>processor rule 9000 (\<open>PROP ?P \<Longrightarrow> PROP ?Q\<close>)
   \<open>fn (ctxt, sequent) => NuApplicant.parser >> (fn thms => fn _ =>
     let open NuBasics
     val apps = NuApplicant.applicant_thms ctxt thms
@@ -2595,7 +2619,7 @@ subsubsection \<open>Constructive\<close>
 
 ML \<open>val phi_synthesis_parsing = Config.declare_bool ("\<phi>_synthesis_parsing", \<^here>) (K false)\<close>
 
-\<phi>processor synthesis 8000 (\<open>\<^bold>c\<^bold>u\<^bold>r\<^bold>r\<^bold>e\<^bold>n\<^bold>t ?blk [?H] \<^bold>r\<^bold>e\<^bold>s\<^bold>u\<^bold>l\<^bold>t\<^bold>s \<^bold>i\<^bold>n ?S\<close> | \<open>?P \<Longrightarrow> PROP ?RM\<close>)
+\<phi>processor synthesis 8000 (\<open>\<^bold>c\<^bold>u\<^bold>r\<^bold>r\<^bold>e\<^bold>n\<^bold>t ?blk [?H] \<^bold>r\<^bold>e\<^bold>s\<^bold>u\<^bold>l\<^bold>t\<^bold>s \<^bold>i\<^bold>n ?S\<close> | \<open>PROP ?P \<Longrightarrow> PROP ?RM\<close>)
   \<open>fn (ctxt, sequent) => Parse.group (fn () => "term") (Parse.inner_syntax (Parse.cartouche || Parse.number))
 >> (fn raw_term => fn () =>
   let
@@ -2662,9 +2686,11 @@ subsubsection \<open>Simplifiers & Reasoners\<close>
 
 \<phi>processor naive_obligation_solver 8000 (\<open>\<^bold>o\<^bold>b\<^bold>l\<^bold>i\<^bold>g\<^bold>a\<^bold>t\<^bold>i\<^bold>o\<^bold>n ?P \<Longrightarrow> PROP ?Q\<close> | \<open>\<^bold>p\<^bold>r\<^bold>e\<^bold>m\<^bold>i\<^bold>s\<^bold>e ?P \<Longrightarrow> PROP ?Q\<close>)
   \<open>fn (ctxt,sequent) => Scan.succeed (fn () =>
-     case Seq.pull (Nu_Reasoners.naive_obligation_solver ctxt sequent)
-       of SOME (ret, _) => (ctxt, ret)
-        | NONE => raise Bypass NONE)\<close>
+    if Config.get ctxt Nu_Reasoner.auto_level >= 2
+    then case Seq.pull (Nu_Reasoners.naive_obligation_solver ctxt sequent)
+           of SOME (ret, _) => (ctxt, ret)
+            | NONE => raise Bypass NONE
+    else raise Bypass NONE)\<close>
 
 \<phi>processor fold 2000 (\<open>PROP ?P\<close>) \<open>
   fn (ctxt, sequent) => NuParse.$$$ "fold" |-- Parse.list1 Parse.thm >> (fn thms => fn _ =>
