notes/exception.md
@@ -1,0 +1,21 @@
+### Exception
+
+{P} C {Q} {E} := (∀x ∈ P. case C x of Success y => y ∈ Q | Exception y => y ∈ E | PartialCorrect => true | Invalid => false)
+
+PartialCorrect means nontermination.
+Invalid means malformed program.
+
+#### Throw
+
+The operation `throw e` first pushes e onto the expression stack, and then returns an exception state.
+`throw e := (push e >> (λs. Exception s))`
+
+The exception object is put on the first element of the expression stack.
+
+#### Catch
+
+The handler is a procedure. This procedure receives the exception object as the first element of the expression stack.
+It should first case-switch the type of the exception object, and call correponding handler for each type.
+
+
+
